changed max line length

src/bundle/Channel.thy
@@ -1,4 +1,4 @@
-(*<*)(*:maxLineLen=78:*)
+(*<*)(*:maxLineLen=69:*)
 theory Channel
 
 imports HOLCF user.Datatypes
@@ -7,29 +7,34 @@ begin
 
 section \<open>Global message type \label{gmt}\<close>
 
-text\<open>Depending on the time model, we allow to transmit slightly different 
-versions of @{type M_pure} messages. In every time slot of the synchronous 
-time model, every channel transmits at most one message. But in every time 
-slot of the general timed model, it is possible to transmit an arbitrary high, 
-but finite number of messages. To allow the usage of both models and also the 
-untimed model, we introduce the M datatype:\<close>
+text\<open>Depending on the time model, we allow to transmit slightly 
+different versions of @{type M_pure} messages. In every time slot of 
+the synchronous time model, every channel transmits at most one 
+message. But in every time slot of the general timed model, it is 
+possible to transmit an arbitrary high, but finite number of 
+messages. To allow the usage of both models and also the untimed
+model, we introduce the M datatype:\<close>
 
-datatype M = Untimed "M_pure" | Timed "M_pure list" | Tsyn "M_pure option"  
-                                                          (* option = tsyn *)
+datatype M = Untimed "M_pure" | 
+             Timed "M_pure list" | 
+             Tsyn "M_pure option"  
+             (* option = tsyn *)
 
 text\<open>We interpret the messages in a time slot of a time model as:
   \<^item> a message, for the untimed model and there is no time slot
-  \<^item> either Some message or None message at all, for the synchronous time model
+  \<^item> either Some message or None message at all, for the synchronous 
+    time model
   \<^item> a finite list of messages, for the timed model
 
 
-In this interpretation a untimed stream can be seen as a special case of a 
-synchronous timed stream (it contains a message in every time slot) and a 
-synchronous timed stream is a special case of a timed stream (it contains at 
-most one element in each list). Now we defined, how a transmitted message in a 
-time slot can look like, respectively to its time model. For this, we define a 
-mapping from channels to sets of elements from M. Obviously, we have to 
-restrict the channels to their time models, else there could be timed and 
+In this interpretation a untimed stream can be seen as a special case
+of a synchronous timed stream (it contains a message in every time 
+slot) and a synchronous timed stream is a special case of a timed 
+stream (it contains at most one element in each list). Now we 
+defined, how a transmitted message in a time slot can look like, 
+respectively to its time model. For this, we define a mapping from 
+channels to sets of elements from M. Obviously, we have to restrict 
+the channels to their time models, else there could be timed and 
 untimed messages on the same channel.\<close>
 
 lemma inj_tsyn[simp]: "inj Tsyn"
@@ -54,23 +59,23 @@ instance M::countable
   by(countable_datatype)
 
 definition ctype::"channel \<Rightarrow> M set" where
-"ctype c \<equiv> if (cMsg c) = {} then {} else 
-  case (cTime c) of TUntimed   \<Rightarrow> Untimed ` (cMsg c) | 
-                   TTimed     \<Rightarrow>  Timed ` {ls. set ls \<subseteq> (cMsg c)} |
-                   TTsyn      \<Rightarrow> Tsyn ` (insert None (Some ` cMsg c))"
-text\<open>This is exactly what @{const ctype} does. It then checks the timing of a 
-channel and then returns the respectively correct set of timeslot messages, 
-where the pure messages depend on @{const cMsg}.
+"ctype c \<equiv> if (cMsg c) = {} then {} else case (cTime c) of 
+                 TUntimed   \<Rightarrow> Untimed ` (cMsg c) | 
+                 TTimed     \<Rightarrow>  Timed ` {ls. set ls \<subseteq> (cMsg c)} |
+                 TTsyn      \<Rightarrow> Tsyn ` (insert None (Some ` cMsg c))"
+text\<open>This is exactly what @{const ctype} does. It then checks the 
+timing of a channel and then returns the respectively correct set of 
+timeslot messages, where the pure messages depend on @{const cMsg}.
   \<^item> Untimed channels can send any message from @{const cMsg}
-  \<^item> Timesynchronous channels can send \<open>Some\<close> message from @{const cMsg} or the 
-    \<open>None\<close> message, interpreted as no Message
-  \<^item> Timed channels can send finite lists, where every list element is in 
-    @{const cMsg}.
+  \<^item> Timesynchronous channels can send \<open>Some\<close> message from 
+    @{const cMsg} or the  \<open>None\<close> message, interpreted as no Message
+  \<^item> Timed channels can send finite lists, where every list element 
+    is in @{const cMsg}.
 
 
-Because we interpret channels without any allowed transmitted messages as no 
-channel at all, we define their @{const ctype} as empty. Hence the following 
-theorems hold.\<close>
+Because we interpret channels without any allowed transmitted 
+messages as no channel at all, we define their @{const ctype} as 
+empty. Hence the following theorems hold.\<close>
 
 theorem ctype_empty_iff: "ctype c = {} \<longleftrightarrow> cMsg c = {}"
   apply(cases "(cTime c)")
@@ -80,38 +85,41 @@ theorem ctype_empty_iff: "ctype c = {} \<longleftrightarrow> cMsg c = {}"
 theorem ctypeempty_ex:"\<exists>c. ctype c = {}"
   by (simp add: cmsgempty_ex ctype_empty_iff)
 
-text\<open>Again, these properties are necessary for defining an empty stream bundle
-\ref{sec:pmsgdata}.\<close>
+text\<open>Again, these properties are necessary for defining an empty 
+stream bundle\ref{sec:pmsgdata}.\<close>
 
 
 section\<open>@{type channel} class definitions\label{chan}\<close>
-text\<open>In this section we restrict the domain of a stream bundle trough the 
-usage of classes. The main Idea is to never construct a stream bundle which 
-has channels with an empty @{const ctype} and channels with non-empty 
-@{const ctype}. With our interpretation of empty bundles, this case would make 
-no sense, because it would be equivalent to the bundle without channels with 
-empty @{const ctype}s. Hence, we restrict the Domain of stream bundles to 
-subsets of the @{type channel} type, where its either possible that every 
-channel transmits a message, or non of the channels can transmit any message 
-at all. We will then use these classes to define the union and subtraction of 
-two domains. This is helpful for combining two stream bundles and hence, 
-necessary for defining the input and output domain of the general composition 
-operator.\<close>
+text\<open>In this section we restrict the domain of a stream bundle trough
+the usage of classes. The main Idea is to never construct a stream 
+bundle which has channels with an empty @{const ctype} and channels 
+with non-empty @{const ctype}. With our interpretation of empty 
+bundles, this case would make no sense, because it would be 
+equivalent to the bundle without channels with empty @{const ctype}s.
+Hence, we restrict the Domain of stream bundles to subsets of the 
+@{type channel} type, where its either possible that every channel 
+transmits a message, or non of the channels can transmit any message
+at all. We will then use these classes to define the union and 
+subtraction of two domains. This is helpful for combining two stream
+bundles and hence, necessary for defining the input and output domain
+of the general composition operator.\<close>
 
 subsection \<open>Preliminaries \<close>
-text\<open>For understandable assumptions in our classes we first define the channel 
-set, that contains all channels with an empty @{const ctype}.\<close>
+text\<open>For understandable assumptions in our classes we first define 
+the channel set, that contains all channels with an empty 
+@{const ctype}.\<close>
 definition cEmpty :: "channel set" where
 "cEmpty = {c. ctype c = {}}"
-text \<open>@{const cEmpty} contains all channels on which no message is allowed to 
-be transmitted.\<close> 
+text \<open>@{const cEmpty} contains all channels on which no message is 
+allowed to be transmitted.\<close> 
 lemma cempty_exists: "cEmpty \<noteq> {}"
   by(simp add: cEmpty_def ctypeempty_ex)
 
 subsection\<open>Class chan\<close>
 text\<open>The following class restricts its type to be injective to our 
-@{type channel} type and to also comply with our main Idea. Through its 
-injectivity, the type is isomorphic to a subset of our @{type channel} type.\<close>
+@{type channel} type and to also comply with our main Idea. Through 
+its injectivity, the type is isomorphic to a subset of our 
+@{type channel} type.\<close>
 
 class chan =
   fixes Rep :: "'a \<Rightarrow> channel"
@@ -122,20 +130,23 @@ class chan =
 begin
 abbreviation "Abs \<equiv> inv Rep"
 end
-text\<open> With @{const Rep} we require a representation function, that maps a type
- of @{class chan} to the @{type channel} type. The first class assumption 
-ensures our channel separation and the second the injectivity. Furthermore, 
-our abstraction function @{const Abs} is the inverse of @{const Rep}.\<close>
+text\<open> With @{const Rep} we require a representation function, that 
+maps a type of @{class chan} to the @{type channel} type. The first 
+class assumption ensures our channel separation and the second the 
+injectivity. Furthermore, our abstraction function @{const Abs} is 
+the inverse of @{const Rep}.\<close>
 
 subsubsection \<open>@{class chan} Functions\<close>
-text\<open>We will now define a function for types of @{class chan}. It returns the 
-Domain of the type. As a result of our class assumptions and of interpreting 
-empty channels as non existing, our domain is empty, if and only if the input 
-type contains channel(s) from @{const cEmpty}. Then we have the empty domain.\<close>
+text\<open>We will now define a function for types of @{class chan}. It 
+returns the Domain of the type. As a result of our class assumptions 
+and of interpreting empty channels as non existing, our domain is 
+empty, if and only if the input type contains channel(s) from 
+@{const cEmpty}. Then we have the empty domain.\<close>
 definition chDom::"'cs::chan itself \<Rightarrow> channel set" where
 "chDom a = (range (Rep::'cs \<Rightarrow> channel)) - cEmpty"
 
-text\<open>The following abbreviation checks, if a type of @{class chan} is empty.\<close>
+text\<open>The following abbreviation checks, if a type of @{class chan} 
+is empty.\<close>
 
 abbreviation chIsEmpty ::"'cs::chan itself \<Rightarrow> bool" where
 "chIsEmpty cs \<equiv> chDom cs = {}"
@@ -145,11 +156,12 @@ lemma inchdom[simp]:"\<not>chIsEmpty TYPE('cs)
   apply(simp add: chDom_def)
   using chan_botsingle by blast
 
-text \<open>As mentioned before, types of @{class chan} can be interpreted as a 
-subset of @{type channel}s, where on every channel either no message can be 
-transmitted, or on every channel some message is allowed to be transmitted. 
-The core theories do not use these classes, but the additional assumptions can
-be useful for the user. Now we define classes for these two options.\<close>
+text \<open>As mentioned before, types of @{class chan} can be interpreted 
+as a subset of @{type channel}s, where on every channel either no 
+message can be transmitted, or on every channel some message is 
+allowed to be transmitted. The core theories do not use these 
+classes, but the additional assumptions can be useful for the user. 
+Now we define classes for these two options.\<close>
 
 subsection\<open>Class somechan\<close>
 class somechan = chan +
@@ -160,12 +172,14 @@ begin
 lemma somechannotempty[simp]:"\<not>chIsEmpty(TYPE('c::somechan))"
   using chDom_def somechan_class.chan_notempty by fastforce
 
-lemma somechandom:"chDom(TYPE('c::somechan)) = range(Rep::'c\<Rightarrow>channel)"
+lemma somechandom:"chDom(TYPE('c::somechan)) 
+                   = range(Rep::'c\<Rightarrow>channel)"
   by(simp add: chDom_def somechan_class.chan_notempty Diff_triv)
 
 end
-text\<open>Types of  @{class somechan} can transmit at least one message on every 
-channel. Hence, we know @{thm somechannotempty} and @{thm somechandom}.\<close>
+text\<open>Types of  @{class somechan} can transmit at least one message on
+every channel. Hence, we know @{thm somechannotempty} and 
+@{thm somechandom}.\<close>
 
 subsection\<open>Class emptychan\<close>
 class emptychan = chan +
@@ -177,15 +191,16 @@ lemma emptychanempty[simp]:"chIsEmpty(TYPE('c::emptychan))"
   by (simp add: chDom_def emptychan_class.chan_empty)
 
 end
-text\<open>Types of @{class emptychan} can not transmit any message on any channel.
-Hence, the Domain is empty @{thm emptychanempty}.\<close>
+text\<open>Types of @{class emptychan} can not transmit any message on any 
+channel. Hence, the Domain is empty @{thm emptychanempty}.\<close>
 
 
 
 section %invisible\<open> rep abs chan lemmata \<close>
 default_sort %invisible chan
 
-lemma repinrange[simp]:"Rep (c::'c) = x \<Longrightarrow> x\<in> range(Rep::'c \<Rightarrow> channel)"
+lemma repinrange[simp]:"Rep (c::'c) = x 
+                        \<Longrightarrow> x\<in> range(Rep::'c \<Rightarrow> channel)"
   by blast
 
 lemma chan_eq[simp]:"Rep (c::'c) = x \<Longrightarrow> x\<in> range(Rep::'d \<Rightarrow> channel) 
@@ -215,23 +230,25 @@ lemma notcdom_empty[simp]:assumes"Rep (c::'c) \<notin>chDom TYPE('c)"
 lemma chdom_in: fixes c::"'cs::chan"
   assumes "chDom TYPE('cs) \<noteq> {}"
     shows "Rep c \<in> chDom TYPE('cs)"
-  by (metis Diff_eq_empty_iff Diff_triv assms chDom_def chan_botsingle rangeI)
+  by (metis Diff_eq_empty_iff Diff_triv assms chDom_def 
+      chan_botsingle rangeI)
 
 
 declare %invisible[[show_types]]
 declare %invisible[[show_consts]]
 
 section \<open>Interconnecting Domain Types\<close>
-text\<open>There are two interesting interconnections between domains. Intuitively, 
-the union operator takes all channels from both domains and the minus operator
-only channels that are in the first, but not the second domain. But because we
-also have to check for channels from @{const cEmpty}, its not that trivial.\<close>
+text\<open>There are two interesting interconnections between domains. 
+Intuitively, the union operator takes all channels from both domains 
+and the minus operator only channels that are in the first, but not 
+the second domain. But because we also have to check for channels 
+from @{const cEmpty}, its not that trivial.\<close>
 
 subsection\<open>Type union operator\<close>
-text\<open>The union of two domains should contain every channel of each domain. So 
-the union of two empty domains should also be empty. But because the type 
-itself can never be empty, we again have to use channels in @{const cEmpty} to
-define the union.\<close> 
+text\<open>The union of two domains should contain every channel of each 
+domain. So the union of two empty domains should also be empty. But 
+because the type itself can never be empty, we again have to use 
+channels in @{const cEmpty} to define the union.\<close> 
 typedef ('c1,'c2) union (infixr "\<union>" 20) = 
         "if chIsEmpty TYPE ('c1) \<and>  chIsEmpty TYPE ('c2) 
             then cEmpty
@@ -239,13 +256,14 @@ typedef ('c1,'c2) union (infixr "\<union>" 20) =
   apply(auto)
   using chDom_def by blast
 
-text\<open>Because we interpret channels in @{const cEmpty} as no real channels, we 
-can define the union of two empty domains as the channel set @{const cEmpty}. 
-The next step is to instantiate the union of two members of class 
-@{class chan} as a member of class @{class chan}. This is rather easy, because 
-either the union results in @{const cEmpty}, so there are only channels where 
-no message can be transmitted, or it results in the union of the domains 
-without channels from @{const cEmpty}. Hence, we can fulfill the class 
+text\<open>Because we interpret channels in @{const cEmpty} as no real 
+channels, we can define the union of two empty domains as the channel
+set @{const cEmpty}. The next step is to instantiate the union of two
+members of class @{class chan} as a member of class @{class chan}. 
+This is rather easy, because either the union results in 
+@{const cEmpty}, so there are only channels where no message can be 
+transmitted, or it results in the union of the domains without 
+channels from @{const cEmpty}. Hence, we can fulfill the class 
 assumptions with the from "typdef" generated representation function 
 @{const Rep_union}.\<close>
 
@@ -259,20 +277,23 @@ instance
   by (simp add: Channel.Rep_union_def Rep_union_inject inj_on_def)
 end
 
-lemma union_range_empty:"chIsEmpty TYPE ('cs1) \<and>  chIsEmpty TYPE ('cs2) \<Longrightarrow> 
-                   range (Rep_union::'cs1 \<union> 'cs2 \<Rightarrow> channel) = cEmpty"
+lemma union_range_empty:"chIsEmpty TYPE ('cs1) 
+                         \<and>  chIsEmpty TYPE ('cs2) \<Longrightarrow> 
+                    range (Rep_union::'cs1 \<union> 'cs2 \<Rightarrow> channel) = 
+                    cEmpty"
   by (metis (mono_tags, lifting) type_definition.Rep_range 
       type_definition_union)
 
-lemma union_range_union:"\<not>(chIsEmpty TYPE ('cs1) \<and>  chIsEmpty TYPE ('cs2)) \<Longrightarrow> 
+lemma union_range_union:"\<not>(chIsEmpty TYPE ('cs1) 
+                         \<and>  chIsEmpty TYPE ('cs2)) \<Longrightarrow> 
                    range (Rep_union::'cs1 \<union> 'cs2 \<Rightarrow> channel) = 
                    chDom TYPE ('cs1) \<union> chDom TYPE('cs2)"
   by (smt type_definition.Rep_range type_definition_union)
 
-text\<open>After the instantiation, class definition like the @{const chDom} 
-function can be used. To verify the correctness of our definition we obtain 
-the domain of the union type and proof, that it is indeed the union of the two
-sub domains.\<close>
+text\<open>After the instantiation, class definition like the 
+@{const chDom} function can be used. To verify the correctness of our
+definition we obtain the domain of the union type and proof, that it 
+is indeed the union of the two sub domains.\<close>
 theorem chdom_union[simp]: "chDom (TYPE('cs1 \<union> 'cs2)) = 
                             chDom (TYPE ('cs1)) \<union> chDom (TYPE('cs2))"
   apply(subst chDom_def)
@@ -280,10 +301,12 @@ theorem chdom_union[simp]: "chDom (TYPE('cs1 \<union> 'cs2)) =
   using chDom_def union_range_empty union_range_union by auto
 
 subsection\<open>Type minus operator\<close>
-text\<open>Subtracting one domain from another results in the empty domain. But 
-analogous to the union, our resulting type always contains channels. 
-Subtracting a set from one of its subsets would result in an empty type. 
-Hence, our result for this case is again @{const cEmpty}.\<close>
+text\<open>Subtracting one domain from another results in the empty domain.
+But analogous to the union, our resulting type always contains 
+channels. Subtracting a set from one of its subsets would result in 
+an empty type. Hence, our result for this case is again 
+@{const cEmpty}.\<close>
+
 typedef ('c1,'c2) minus (infixr "-" 20) = 
         "(if chDom TYPE('c1) \<subseteq> chDom TYPE('c2) 
              then cEmpty
@@ -291,8 +314,8 @@ typedef ('c1,'c2) minus (infixr "-" 20) =
 apply(cases "range Rep \<subseteq> range Rep", auto)
   using cempty_exists by blast+
 
-text\<open>Instantiating the subtraction result of two @{class chan} types is also 
-in the class. The proof is, like above, straight forward.\<close>
+text\<open>Instantiating the subtraction result of two @{class chan} types
+is also in the class. The proof is, like above, straight forward.\<close>
 instantiation minus :: (chan, chan) chan
 begin
 definition "Rep == Rep_minus"
@@ -305,7 +328,7 @@ end
 
 
 lemma minus_range_empty:"chDom TYPE('cs1) \<subseteq> chDom TYPE('cs2) \<Longrightarrow> 
-                   range (Rep_minus::'cs1 - 'cs2 \<Rightarrow> channel) = cEmpty"
+                  range (Rep_minus::'cs1 - 'cs2 \<Rightarrow> channel) = cEmpty"
   by (metis (mono_tags, lifting) type_definition.Rep_range 
       type_definition_minus)
 
@@ -315,16 +338,17 @@ lemma minus_range_minus:"\<not>(chDom TYPE('cs1) \<subseteq> chDom TYPE('cs2)) \
   by (metis (mono_tags, lifting) type_definition.Rep_range 
       type_definition_minus)
 
-text\<open>For verifying the minus operator we again take a look at the resulting 
-domain in the following theorem.\<close>
+text\<open>For verifying the minus operator we again take a look at the
+resulting domain in the following theorem.\<close>
 theorem chdom_minus[simp]: "chDom (TYPE('cs1 - 'cs2)) = 
                             chDom (TYPE ('cs1)) - chDom (TYPE('cs2))"
   apply(subst chDom_def)
   apply(simp_all add: Rep_minus_def)
   using Diff_Int_distrib2 minus_range_empty minus_range_minus by auto
  
-text\<open>If we subtract domain \<open>A\<close> from domain \<open>B\<close> the resulting domain should 
-contain no channels from \<open>A\<close>.We also verify this correctness property.\<close>
+text\<open>If we subtract domain \<open>A\<close> from domain \<open>B\<close> the resulting domain 
+should contain no channels from \<open>A\<close>.We also verify this correctness
+property.\<close>
 theorem [simp]:"chDom (TYPE('cs1 - 'cs2)) \<inter> chDom (TYPE ('cs2)) = {}"
   by auto
 
