src/bundle/sbElem.thy
@@ -1,4 +1,4 @@
-(*<*)(*:maxLineLen=78:*)
+(*<*)(*:maxLineLen=69:*)
 theory sbElem
   imports Channel
 begin
@@ -13,22 +13,25 @@ section \<open> mono2mono\<close>
 named_theorems mono2mono "monofun intro rule"
 *)
 section \<open>sbElem\<close>
-text\<open>A function from channels to messages is quite useful in our later 
-theories. Hence, we define a the sbElem type. But the possibility to have no 
-@{type channel}s in the @{const chDom} of a @{class chan} type, forces us to use 
-the allow  @{const None} function in such a case.\<close>
+text\<open>A function from channels to messages is quite useful in our 
+later theories. Hence, we define a the sbElem type. But the 
+possibility to have no @{type channel}s in the @{const chDom} of a 
+@{class chan} type, forces us to use the allow  @{const None} 
+function in such a case.\<close>
 
 subsection \<open>sbElem Definition \<close>
 fun sbElem_well :: "('c \<Rightarrow> M) option \<Rightarrow> bool" where
 "sbElem_well None = chIsEmpty(TYPE('c))" |
-"sbElem_well (Some sbe) = (\<forall> c. sbe c \<in> ctype ((Rep::'c\<Rightarrow>channel) c))" 
-(* cbot ist leer, daher wird das nie wahr sein für das leere Bündel *)
-text\<open>Predicate @{const sbElem_well} is used to define sbElem and only allows 
-functions with a Message on each channel that are allowed to be transmitted 
-(@{const ctype}), or no function, if the channel type is empty.\<close>
+"sbElem_well (Some sbe) = (\<forall> c. sbe c \<in> ctype((Rep::'c\<Rightarrow>channel) c))" 
+(*cbot ist leer, daher wird das nie wahr sein für das leere Bündel *)
+text\<open>Predicate @{const sbElem_well} is used to define sbElem and only
+allows functions with a Message on each channel that are allowed to 
+be transmitted (@{const ctype}), or no function, if the channel type 
+is empty.\<close>
 
 text\<open>Type sbElem is can be interpreted as a Timeslice.\<close>
-typedef 'c sbElem ("(_\<^sup>\<surd>)" [1000] 999) = "{f::('c \<Rightarrow> M) option. sbElem_well f}"
+typedef 'c sbElem ("(_\<^sup>\<surd>)"[1000] 999) = 
+        "{f::('c \<Rightarrow> M) option. sbElem_well f}"
 proof(cases "chIsEmpty(TYPE('c))")
   case True
   then show ?thesis
@@ -38,7 +41,8 @@ next
   case False
   then have "\<forall>c\<in>(range (Rep::'c\<Rightarrow>channel)). ctype c \<noteq> {}"
     using cEmpty_def chDom_def chan_botsingle by blast
-  then have "sbElem_well (Some(\<lambda>(c::'c). (SOME m. m \<in> ctype (Rep c))))"
+  then have "sbElem_well 
+             (Some(\<lambda>(c::'c). (SOME m. m \<in> ctype (Rep c))))"
     apply(simp add: sbElem_well.cases,auto)
     by (simp add: some_in_eq)
   then show ?thesis
@@ -73,50 +77,53 @@ lemma sbtypeepmpty_sbenone[simp]:"chIsEmpty TYPE ('cs)
                                   \<Longrightarrow> (sbe::'cs\<^sup>\<surd>) = Abs_sbElem(None)"
   apply(simp add: chDom_def)
   apply(rule sbe_eqI)
-  by (metis Diff_eq_empty_iff not_Some_eq Rep_sbElem mem_Collect_eq chDom_def 
-      sbtypeempty_notsbewell)
+  by (metis Diff_eq_empty_iff not_Some_eq Rep_sbElem mem_Collect_eq 
+      chDom_def sbtypeempty_notsbewell)
 
 lemma sbtypenotempty_somesbe:"\<not>(chIsEmpty TYPE ('c)) 
                               \<Longrightarrow>\<exists>f::'c \<Rightarrow> M. sbElem_well (Some f)"
   apply(rule_tac x="(\<lambda>(c::'c). (SOME m. m \<in> ctype (Rep c)))" in exI)
-  apply(simp add: chDom_def cEmpty_def sbElem_well.cases some_in_eq,auto)
+  apply(simp add: chDom_def cEmpty_def sbElem_well.cases some_in_eq)
   using cEmpty_def chan_botsingle by blast
 
 setup_lifting %invisible type_definition_sbElem
 (*<*) (*Not in pdf at the moment, because ugly*)
 subsection \<open>sbElem functions\<close>
 
-text\<open>This function retrieves an element on channel e from the sbElem. This 
-only works if Elements are allowed on channel e and channel e is also in 
-type c.\<close>
+text\<open>This function retrieves an element on channel e from the sbElem.
+This only works if Elements are allowed on channel e and channel e is
+also in type c.\<close>
 (*works if sbe \<noteq> None* and 'e \<subseteq> 'c *)
 definition sbegetch::"'e \<Rightarrow> 'c\<^sup>\<surd> \<Rightarrow> M"where 
 "sbegetch c = (\<lambda> sbe. ((the (Rep_sbElem sbe)) (Abs (Rep c))))"
 
 
-lemma sbtypenotempty_fex[simp]:"\<not>(chIsEmpty TYPE ('cs)) 
-                                \<Longrightarrow> \<exists>f. Rep_sbElem (sbe::'cs\<^sup>\<surd>) = (Some f)"
+lemma sbtypenotempty_fex[simp]:
+"\<not>(chIsEmpty TYPE ('cs)) \<Longrightarrow> \<exists>f. Rep_sbElem (sbe::'cs\<^sup>\<surd>) = (Some f)"
   apply(rule_tac x="(\<lambda>(c::'c). (THE m. m= sbegetch c sbe))" in exI)
   apply(simp add: sbegetch_def)
   by (metis option.collapse sbElem_well.simps(1) sbelemwell2fwell)
 
-text\<open>This function Converts the Domain of an sbElem. This works if the Domain 
-it converts to, is smaller or equal\<close>
+text\<open>This function Converts the Domain of an sbElem. This works if 
+the Domain it converts to, is smaller or equal\<close>
 definition sbeConvert::"'c\<^sup>\<surd> \<Rightarrow> 'd\<^sup>\<surd>"where
 "sbeConvert = (\<lambda>sbe. Abs_sbElem(Some (\<lambda>c. sbegetch c sbe)))"
 
 lemma chIsEmpty2chIsEmpty:"chIsEmpty TYPE ('c) \<Longrightarrow> 
   Rep (c::'c) \<in> range(Rep::'d\<Rightarrow> channel) \<Longrightarrow> chIsEmpty TYPE ('d)"
   apply(simp add: chDom_def cEmpty_def,auto)
-  by (metis (mono_tags, lifting) Int_Collect cEmpty_def chan_botsingle 
-      insert_not_empty le_iff_inf mk_disjoint_insert repinrange)
+  by (metis (mono_tags, lifting) Int_Collect cEmpty_def 
+      chan_botsingle insert_not_empty le_iff_inf mk_disjoint_insert
+      repinrange)
 
-lemma sbgetch_ctype: assumes "Rep (c::'e) \<in> range(Rep::'d \<Rightarrow> channel)" 
-                     and "\<not>chIsEmpty(TYPE('d))"
+lemma sbgetch_ctype: 
+  assumes "Rep (c::'e) \<in> range(Rep::'d \<Rightarrow> channel)" 
+  and "\<not>chIsEmpty(TYPE('d))"
   shows "sbegetch c (sbe2::'d\<^sup>\<surd>) \<in> ctype ((Rep::'e \<Rightarrow> channel) c)"
   using assms apply(simp add: sbegetch_def)
-  by (metis (no_types, hide_lams) assms(1) assms(2) f_inv_into_f option.sel 
-      sbElem_well.simps(2) sbegetch_def sbelemwell2fwell sbtypenotempty_fex)
+  by (metis (no_types, hide_lams) assms(1) assms(2) f_inv_into_f 
+      option.sel sbElem_well.simps(2) sbegetch_def sbelemwell2fwell
+      sbtypenotempty_fex)
 
 lemma sberestrict_getch:
   assumes"Rep (c::'c) \<in> range(Rep::'d \<Rightarrow> channel)"
@@ -127,12 +134,14 @@ lemma sberestrict_getch:
   apply(simp add: sbeConvert_def)
   apply(simp add: sbegetch_def)
   apply(subst Abs_sbElem_inverse)
-  apply (smt Rep_sbElem chDom_def f_inv_into_f mem_Collect_eq option.sel 
-         rangeI sbElem_well.elims(1) sbElem_well.simps(2) subset_iff)
+  apply (smt Rep_sbElem chDom_def f_inv_into_f mem_Collect_eq 
+         option.sel rangeI sbElem_well.elims(1) sbElem_well.simps(2)
+         subset_iff)
   by simp
   
 
-text\<open>This unites two sbElems. It works, if type e is a subset of the union of 
+text\<open>This unites two sbElems. It works, if type e is a subset of the 
+     union of 
      type c and d. First sbElem has priority\<close>
 definition sbeUnion::"'c\<^sup>\<surd> \<Rightarrow> 'd\<^sup>\<surd> \<Rightarrow> 'e\<^sup>\<surd>"where
 "sbeUnion = (\<lambda>sbe1 sbe2. Abs_sbElem (Some(\<lambda> c. 
@@ -152,7 +161,8 @@ lemma sbeunion_getchfst:
   apply (auto simp add: chDom_def assms)
   using assms(2) sbgetch_ctype apply force
   apply (smt assms(2) sbElem_well.simps(2) Un_iff assms(1) assms(3) 
-         chIsEmpty2chIsEmpty chan_eq repinrange sbgetch_ctype subset_eq)
+         chIsEmpty2chIsEmpty chan_eq repinrange sbgetch_ctype 
+         subset_eq)
   by(simp add: sbegetch_def assms)
 
 
@@ -162,13 +172,16 @@ lemma sbeunion_getchsnd:
   and "\<not>(chIsEmpty TYPE('d))"
   and "range(Rep::'e \<Rightarrow> channel) \<subseteq> 
        range(Rep::'c \<Rightarrow> channel) \<union> range(Rep::'d \<Rightarrow> channel)"
-  shows"sbegetch c ((sbeUnion::'c\<^sup>\<surd> \<Rightarrow> 'd\<^sup>\<surd> \<Rightarrow> 'e\<^sup>\<surd>) sbe1 sbe2) = sbegetch c sbe2"
+shows"sbegetch c ((sbeUnion::'c\<^sup>\<surd> \<Rightarrow> 'd\<^sup>\<surd> \<Rightarrow> 'e\<^sup>\<surd>) sbe1 sbe2) = 
+      sbegetch c sbe2"
   apply(simp add: sbeUnion_def sbegetch_def)
   apply(subst Abs_sbElem_inverse)
   apply (auto simp add: chDom_def assms)
-  apply (metis assms(1) assms(3) chIsEmpty2chIsEmpty chan_eq rangeI sbgetch_ctype)
+  apply (metis assms(1) assms(3) chIsEmpty2chIsEmpty chan_eq rangeI 
+         sbgetch_ctype)
   apply (smt assms sbElem_well.simps(2) Un_iff assms(1) assms(3) 
-         chIsEmpty2chIsEmpty chan_eq repinrange sbgetch_ctype subset_eq)
+         chIsEmpty2chIsEmpty chan_eq repinrange sbgetch_ctype 
+         subset_eq)
   by(simp add: sbegetch_def assms)
 (*>*)
 
